examples/Simple_Time_Prog.thy
@@ -1,11 +1,17 @@
+section \<open> Simple Time Programs \<close>
+
 theory Simple_Time_Prog
   imports Simple_Time_Theory
 begin
+
+text \<open> A timed program type is created, corresponding to the healthy timed relations. \<close>
 
 typedef 's tprog = "{P :: 's time_rel. P is HT}"
   using Delay_HT by blast
 
 setup_lifting type_definition_tprog
+
+text \<open> We can also show the other operators can be lifted to operate over the new type. \<close>
 
 lift_definition Delay :: "nat \<Rightarrow> 's tprog" is "Simple_Time_Theory.Delay" by (simp add: Delay_HT)
 
